expose pts_to_not_null as an action

pulse/lib/pulse_core/PulseCore.Heap.fst
@@ -1094,6 +1094,18 @@ let gather_action #a #pcm r v0 v1
     in
     refined_pre_action_as_action g
 
+
+////////////////////////////////////////////////////////////////////////////////
+let pts_to_not_null_action #a #pcm r v
+  = let g : refined_pre_action (pts_to r v)
+                               (squash (not (is_null r)))
+                               (fun _ -> pts_to r v)
+      = fun m ->
+          pts_to_not_null r v m;
+          (| (), m |)
+    in
+    refined_pre_action_as_action g
+    
 ////////////////////////////////////////////////////////////////////////////////
 #push-options "--z3rlimit 20"
 let extend #a #pcm x addr h =
